src/Tree_stack.thy
@@ -3,45 +3,8 @@ imports Tree
 begin
 
 (*begin focus definition*)
-datatype One_or_two = 
-Inserting_one "Tree"
-| Inserting_two "Tree * key * Tree"
-
-type_synonym inserting_two_t =  "Tree * key * Tree"
-
-type_synonym ins_focus_t = One_or_two
-(*end focus definition*)
-
 datatype 'f focus_t = Focus 'f
-
-definition split_node :: "node_t \<Rightarrow> inserting_two_t" where
-"split_node n == (
-let (l,cs) = n in
-let n0 = min_node_keys in
-let left_ks = take n0 l in
-let (k,right_ks) = (case drop n0 l of (k#ks) \<Rightarrow> (k,ks)) in
-let left_rs = take (1+n0) cs in
-let right_rs = drop (1+n0) cs in
-(Node(left_ks,left_rs),k,Node(right_ks,right_rs))
-)"
-
-definition update_focus_at_position :: "node_t \<Rightarrow> nat \<Rightarrow> ins_focus_t \<Rightarrow> ins_focus_t" where
-"update_focus_at_position n i f == (
-let (ks,rs) = n in
-case f of
-Inserting_one t \<Rightarrow> (
-let rs2 = dest_Some(list_replace_1_at_n rs i t) in
-Inserting_one(Node(ks,rs2)))
-| Inserting_two (tl_,k,tr) \<Rightarrow> (
-let ks2 = list_insert_at_n ks i [k] in
-let rs2 = list_replace_at_n rs i [tl_,tr] |> dest_Some in
-case (length ks2 \<le> max_node_keys) of
-True \<Rightarrow> Inserting_one(Node(ks2,rs2))
-| False \<Rightarrow> (
-Inserting_two(split_node(ks2,rs2))
-)
-)
-)"
+(*end focus definition*)
 
 (*begin context definition*)
 type_synonym left_bound = "key option"
@@ -104,22 +67,4 @@ wellformed_context_1 (Rmbs False) x1
 
 definition dest_ts :: "'f tree_stack \<Rightarrow> 'f * context_t" where
 "dest_ts ts == (case ts of Tree_stack((Focus f),c) \<Rightarrow> (f,c))"
-
-
-definition step_tree_stack :: "'f tree_stack \<Rightarrow> ('f tree_stack) option" where
-"step_tree_stack ts == (
-let (f,stk) = dest_ts ts in
-case stk of 
-Nil \<Rightarrow> None
-| ((lb,(n,i),rb)#xs) \<Rightarrow> (
-let f2 = update_focus_at_position n i f in
-Some(Tree_stack((Focus f2),xs))
-)
-
-)
-
-"
-
-declare [[code abort: key_lt key_le min_node_keys max_node_keys]]
-export_code step_tree_stack in Scala module_name Insert_tree_stack file "/tmp/Insert_tree_stack.scala"
 end
